pulse/share/pulse/examples/dice/l0/L0Types.fst
@@ -15,16 +15,3 @@
 *)
 
 module L0Types
-open Pulse.Lib.Pervasives
-
-let x509_version_t : Type0 = UInt32.t
-
-let x509_serialNumber_t : Type0 = UInt32.t
-
-let deviceIDCRI_t : Type0 = UInt32.t
-
-let deviceIDCSR_t : Type0 = UInt32.t
-
-let aliasKeyTBS_t : Type0 = UInt32.t
-
-let aliasKeyCRT_t : Type0 = UInt32.t
